Incremental/LessBusy.lean
@@ -1,6 +1,6 @@
 module
 
-public import Incremental.Parametric
+public import Incremental.Basic
 
 namespace Incremental
 
@@ -11,25 +11,25 @@ namespace LessBusy
 variable
   {ℭ : BuildConfig}
   [BEq ℭ.Q] [LawfulBEq ℭ.Q] [Hashable ℭ.Q]
-  (tasks : MTasks ℭ) (ι₀ : ∀ i, ℭ.V i)
+  (tasks : Tasks ℭ) (ι₀ : ∀ i, ℭ.V i)
 
-abbrev VCache := DHashMap ℭ.Q (Value Id.instMonad tasks ι₀)
+abbrev VCache := DHashMap ℭ.Q (Value tasks ι₀)
 
-def action : Task.Monad.Action (StateM (VCache tasks ι₀)) Id where
+def action : MonadAction (StateM (VCache tasks ι₀)) Id where
   rel P m b := ∀ s, P (m.run' s) b
   rel_pure hab _ := hab
   rel_bind hma hk s := hk _ _ (hma s) _
 
 def run (q₀ : ℭ.Q)
     (fetch : ∀ q, ℭ.rel q q₀ →
-      StateM (VCache tasks ι₀) (Value Id.instMonad tasks ι₀ q)) :
-    StateM (VCache tasks ι₀) (Value Id.instMonad tasks ι₀ q₀) := do
+      StateM (VCache tasks ι₀) (Value tasks ι₀ q)) :
+    StateM (VCache tasks ι₀) (Value tasks ι₀ q₀) := do
   let ⟨r, hr⟩ ← MonadAttach.attach ((tasks q₀).fn (StateM (VCache tasks ι₀))
     (fun i => StateT.pure (ι₀ i))
     (fun q hq => Value.val <$> fetch q hq))
-  have : r = computeM tasks ι₀ q₀ := by
+  have : r = compute tasks ι₀ q₀ := by
     have ⟨s, s', heq⟩ := hr
-    have hft := MTasks.freeTheorem tasks q₀ (action tasks ι₀)
+    have hft := Tasks.freeTheorem tasks q₀ (action tasks ι₀)
       ι₀
       (fun i => StateT.pure (ι₀ i))
       (fun q hq => Value.val <$> fetch q hq)
@@ -39,7 +39,7 @@ def run (q₀ : ℭ.Q)
   return ⟨r, this⟩
 
 def fetch (q₀ : ℭ.Q) :
-    StateM (VCache tasks ι₀) (Value Id.instMonad tasks ι₀ q₀) := do
+    StateM (VCache tasks ι₀) (Value tasks ι₀ q₀) := do
   if let some v := (← get).get? q₀ then return v
   let v ← run tasks ι₀ q₀ (fun q _ => fetch q)
   modify (·.insert q₀ v)
@@ -53,8 +53,7 @@ variable
   (J : Type) [Input ℭ J]
   [BEq ℭ.Q] [LawfulBEq ℭ.Q] [Hashable ℭ.Q]
 
-public def LessBusy (tasks : MTasks ℭ) : Build Monad ℭ J tasks Id Id where
-  cId := Id.instMonad
+public def LessBusy (tasks : Tasks ℭ) : Build ℭ J tasks Id Id where
   σ := J
   init := id
   inputs := Input.get
