Incremental/Busy.lean
@@ -8,14 +8,13 @@ variable
   (ℭ : BuildConfig)
   (J : Type) [Input ℭ J]
 
-public def Busy {c : (Type → Type) → Type 1} (cId : c Id) (tasks : Tasks c ℭ) :
-    Build c ℭ J tasks Id Id where
-  cId := cId
+public def Busy (tasks : Tasks ℭ) :
+    Build ℭ J tasks Id Id where
   σ := J
   init := id
   inputs := Input.get
   set i v := modify fun store => Input.set store i v
   build q store :=
-    (⟨compute cId tasks (Input.get store) q, rfl⟩, store)
+    (⟨compute tasks (Input.get store) q, rfl⟩, store)
 
 end Incremental
