Incremental/Shake/C.lean
@@ -12,7 +12,7 @@ variable
   [BEq ℭ.I] [LawfulBEq ℭ.I] [Hashable ℭ.I] [∀ i, Hashable (ℭ.V i)]
   [BEq ℭ.Q] [LawfulBEq ℭ.Q] [Hashable ℭ.Q] [∀ q, Hashable (ℭ.R q)]
 
-instance : Inhabited (Tasks Monad ℭ → ∀ q, ShakeRT.Store ℭ J → ℭ.R q × ShakeRT.Store ℭ J) :=
+instance : Inhabited (Tasks ℭ → ∀ q, ShakeRT.Store ℭ J → ℭ.R q × ShakeRT.Store ℭ J) :=
   ⟨sorry⟩
 
 @[extern "lean_shake_build"]
@@ -21,11 +21,11 @@ public opaque shakeCBuild
     [BEq ℭ.I] [Hashable ℭ.I] [∀ i, Hashable (ℭ.V i)]
     [BEq ℭ.Q] [Hashable ℭ.Q] [∀ q, Hashable (ℭ.R q)]
     {J : Type} [Input ℭ J] :
-    Tasks Monad ℭ → ∀ q,
+    Tasks ℭ → ∀ q,
     ShakeRT.Store ℭ J → ℭ.R q × ShakeRT.Store ℭ J
 
-@[expose] public def ShakeC (tasks : Tasks Monad ℭ) : Build Monad ℭ J tasks Id Id where
-  cId := Id.instMonad
+@[expose] public def ShakeC (tasks : Tasks ℭ) : Build ℭ J tasks Id Id where
+
   σ := ShakeRT.Store ℭ J
   init inputs := {
     inputs
